secure_api/box/functor_box/Box.Flags.fsti
@@ -1,0 +1,38 @@
+(**
+   This module contains flags that control the idealization of encryption and decryption,
+   both of AE and of PKE. The flags indicate whether certain assumption are assumed to be
+   true or not. Also, the refinements on the flag type indicate implications between the
+   assumptions such as ae_ind_cpa /\ ae_int_ctxt ==> ae_ind_cca.
+   Note, that for purposes of type-checking, the flags are not set. This
+   ensures that the program is well typed for any permutation of set flags (that is permissible
+   by the refinements).
+*)
+module Box.Flags
+
+//abstract type flags_module =
+//  | FM:
+//    prf_odh: bool ->
+//    ae_int_ctxt: bool ->
+//    ae_ind_cpa : (b:bool{b ==> ae_int_ctxt}) ->
+//    ae_ind_cca : (b:bool{b <==> (b2t ae_ind_cpa /\ ae_int_ctxt)}) ->
+//    pkae_int_ctxt : (b:bool{b <==> ae_int_ctxt}) ->
+//    pkae_ind_cpa : (b:bool{b <==> b2t ae_ind_cpa}) ->
+//    pkae : (b:bool{b ==> (((b2t ae_ind_cca) /\ prf_odh) /\ (b2t pkae_int_ctxt /\ b2t pkae_ind_cpa))}) ->
+//    state : (b:bool{b2t ae_ind_cca \/ prf_odh ==> b}) ->
+//    flags_module
+
+val prf_odh : bool
+
+val ae_int_ctxt : bool
+
+val ae_ind_cpa : b:bool{b ==> ae_int_ctxt} // ae_int_ctxt needs to be idealized before ae_ind_cpa
+
+val ae_ind_cca : b:bool{b <==> (b2t ae_ind_cpa /\ ae_int_ctxt)}
+
+val pkae_int_ctxt : b:bool{b <==> ae_int_ctxt}
+
+val pkae_ind_cpa : b:bool{b <==> b2t ae_ind_cpa}
+
+val pkae : b:bool{b ==> (((b2t ae_ind_cca) /\ prf_odh) /\ (b2t pkae_int_ctxt /\ b2t pkae_ind_cpa))}
+
+val state : b:bool{b2t ae_ind_cca \/ prf_odh ==> b}
