secure_api/box/functor_box/Box.Indexing.fst
@@ -1,0 +1,193 @@
+(**
+   This module contains functions and various lemmas concerning indices. Indices (ids) are used to link keys and plaintexts to a
+   certain instance in the cryptographic model. This module also contains tables to reflect freshness and honesty of ids.
+   TODO: Remove all state from this module.
+   * move honesty information into the AE and DH module
+   * use "registered" instead of fresh
+   * remove unused lemmas
+   * get rid of the assumes
+*)
+module Box.Indexing
+
+open FStar.Set
+open FStar.Seq
+open FStar.HyperHeap
+open FStar.HyperStack
+open FStar.HyperStack.ST
+
+open Box.Flags
+
+module MR = FStar.Monotonic.RRef
+module MM = MonotoneMap
+module Curve = Spec.Curve25519
+
+
+type id_log_region = (r:MR.rid{extends r root /\ is_eternal_region r /\ is_below r root})
+
+type honesty =
+  | UNDEFINED
+  | HONEST
+  | DISHONEST
+
+type id_log_value = honesty
+let id_log_range = fun id_log_key -> id_log_value
+let id_log_inv (id_log_kt:Type0) (m:MM.map' id_log_kt id_log_range) = True
+
+type id_log_t (rgn:id_log_region) (id_log_kt:Type0) = MM.t rgn id_log_kt id_log_range (id_log_inv id_log_kt)
+
+abstract noeq type index_module =
+  | IM:
+    rgn: (id_log_region) ->
+    subId: (t:Type0{hasEq t}) -> // express that there is a total order on ids
+    compose_ids: (subId -> subId -> (subId*subId)) ->
+    id_log: (id_log_t rgn subId) ->
+    index_module
+
+
+type id (im:index_module) = i:(im.subId*im.subId) // add refinement once total order on subids is established{fst i <= snd i}
+
+noeq type meta_id (im:index_module) =
+  | ID of id im
+  | SUBID of im.subId
+
+// Anything below here should probably be in the "user-module"
+#set-options "--z3rlimit 300 --max_ifuel 1 --max_fuel 1"
+assume val symmetric_id_generation (im:index_module): i1:im.subId -> i2:im.subId -> Lemma
+  (requires (True))
+  (ensures (forall id1 id2. im.compose_ids id1 id2 = im.compose_ids id2 id1))
+  [SMTPat (im.compose_ids i1 i2)]
+//let symmetric_id_generation i1 i2 = ()
+
+private let measure_id (im:index_module) (i:meta_id im) =
+  match i with
+  | SUBID i' -> 0
+  | _ -> 1
+
+val registered: (im:index_module) -> (i:meta_id im) -> Tot Type0 (decreases (measure_id im i))
+let rec registered (im:index_module) (i:meta_id im) =
+  match i with
+  | SUBID i' -> MR.witnessed (MM.defined im.id_log i')
+  | ID (i1,i2) -> registered im (SUBID i1) /\ registered im (SUBID i2)
+
+// Put the correct flag here, as soon as we have flags for proof steps
+val honest: (im:index_module) -> (i:meta_id im) -> Tot (t:Type0{t ==> registered im i}) (decreases (measure_id im i))
+let rec honest (im:index_module) (i:meta_id im) =
+  match i with
+  | SUBID i' -> MR.witnessed (MM.contains im.id_log i' HONEST) /\ MR.witnessed (MM.defined im.id_log i')
+  | ID (i1,i2) -> honest im (SUBID i1) /\ honest im (SUBID i2)
+
+val dishonest: (im:index_module) -> (i:meta_id im) -> Tot (t:Type0{(t /\ SUBID? i) ==> registered im i}) (decreases (measure_id im i))
+let rec dishonest im i =
+  match i with
+  | SUBID i' -> MR.witnessed (MM.contains im.id_log i' DISHONEST) /\ MR.witnessed (MM.defined im.id_log i')
+  | ID (i1,i2) -> dishonest im (SUBID i1) \/ dishonest im (SUBID i2)
+
+val undefined: (im:index_module) -> (i:meta_id im) -> Tot (t:Type0{(t /\ SUBID? i) ==> registered im i}) (decreases (measure_id im i))
+let rec undefined im i =
+  match i with
+  | SUBID i' -> MR.witnessed (MM.contains im.id_log i' UNDEFINED) /\ MR.witnessed (MM.defined im.id_log i')
+  | ID (i1,i2) -> (undefined im (SUBID i1) /\ honest im (SUBID i2))
+                 \/ (honest im (SUBID i1) /\ undefined im (SUBID i2))
+                 \/ (undefined im (SUBID i1) /\ undefined im (SUBID i2))
+
+
+type absurd_honest (im:index_module) (i:meta_id im{registered im i /\ (undefined im i \/ dishonest im i)}) = honest im i
+type absurd_dishonest (im:index_module) (i:meta_id im{registered im i /\ (undefined im i \/ honest im i)}) = dishonest im i
+type absurd_undefined (im:index_module) (i:meta_id im{registered im i /\ (honest im i \/ dishonest im i)}) = undefined im i
+assume val lemma_honest_and_others_tot: im:index_module -> i:meta_id im{registered im i /\ (undefined im i \/ dishonest im i)} -> absurd_honest im i -> Lemma (False)
+assume val lemma_dishonest_and_others_tot: im:index_module -> i:meta_id im{registered im i /\ (undefined im i \/ honest im i)} -> absurd_dishonest im i -> Lemma (False)
+assume val lemma_undefined_and_others_tot: im:index_module -> i:meta_id im{registered im i /\ (honest im i \/ dishonest im i)} -> absurd_undefined im i -> Lemma (False)
+
+
+val lemma_dishonest_not_others: (im:index_module) -> (i:meta_id im) -> ST unit
+  (requires (fun h0 ->
+    registered im i
+    /\ dishonest im i
+  ))
+  (ensures (fun h0 _ h1 ->
+    ~(honest im i)
+    /\ ~(undefined im i)
+    /\ h0==h1
+  ))
+let lemma_dishonest_not_others im i =
+  let (j:(i:meta_id im{registered im i /\ dishonest im i})) = i in
+  FStar.Classical.impl_intro (lemma_honest_and_others_tot im j);
+  FStar.Classical.impl_intro (lemma_undefined_and_others_tot im j);
+  assert((honest im i \/ undefined im i)==> False)
+
+val lemma_honest_not_others: (im:index_module) -> (i:meta_id im) -> ST unit
+  (requires (fun h0 ->
+    registered im i
+    /\ honest im i
+  ))
+  (ensures (fun h0 _ h1 ->
+    ~(dishonest im i)
+    /\ ~(undefined im i)
+    /\ h0==h1
+  ))
+let lemma_honest_not_others im i =
+  let (j:(i:meta_id im{registered im i /\ honest im i})) = i in
+  FStar.Classical.impl_intro (lemma_dishonest_and_others_tot im j);
+  FStar.Classical.impl_intro (lemma_undefined_and_others_tot im j);
+  assert((dishonest im i \/ undefined im i) ==> False)
+
+val lemma_undefined_not_others: (im:index_module) -> (i:meta_id im) -> ST unit
+  (requires (fun h0 ->
+    registered im i
+    /\ undefined im i
+  ))
+  (ensures (fun h0 _ h1 ->
+    ~(dishonest im i)
+    /\ ~(honest im i)
+    /\ h0==h1
+  ))
+let lemma_undefined_not_others im i =
+  let (j:(i:meta_id im{registered im i /\ undefined im i})) = i in
+  FStar.Classical.impl_intro (lemma_dishonest_and_others_tot im j);
+  FStar.Classical.impl_intro (lemma_honest_and_others_tot im j);
+  assert((dishonest im i \/ honest im i) ==> False)
+
+let merge_honesty_states h1 h2 =
+  match h1,h2 with
+  | HONEST,HONEST -> HONEST
+  | _,DISHONEST -> DISHONEST
+  | DISHONEST,_ -> DISHONEST
+  | _,_ -> UNDEFINED
+
+#set-options "--z3rlimit 500 --max_ifuel 2 --max_fuel 2"
+val get_honesty: im:index_module -> i:meta_id im{registered im i} -> ST(h:honesty{(HONEST? h <==> (honest im i)) /\ (DISHONEST? h <==> dishonest im i) /\ (UNDEFINED? h <==> undefined im i)}) (decreases (measure_id im i))
+  (requires (fun h0 -> True))
+  (ensures (fun h0 b h1 ->
+    modifies_none h0 h1
+    /\ h0==h1
+  ))
+let rec get_honesty im i =
+  MR.m_recall im.id_log;
+  match i with
+  | SUBID i' ->
+    (MR.testify (MM.defined im.id_log i');
+    match MM.lookup im.id_log i' with
+    |Some h ->
+      (match h with
+      | HONEST ->
+        lemma_honest_not_others im i;
+        h
+      | DISHONEST ->
+        lemma_dishonest_not_others im i;
+        h
+      | UNDEFINED ->
+        lemma_undefined_not_others im i;
+        h))
+  | ID (i1,i2) ->
+    let h1 = get_honesty im (SUBID i1) in
+    let h2 = get_honesty im (SUBID i2) in
+    match merge_honesty_states h1 h2 with
+    | HONEST ->
+      lemma_honest_not_others im i;
+      HONEST
+    | DISHONEST ->
+      lemma_dishonest_not_others im i;
+      DISHONEST
+    | UNDEFINED ->
+      lemma_undefined_not_others im i;
+      UNDEFINED
