secure_api/box/functor_box/Box.Key.fst
@@ -1,0 +1,142 @@
+(**
+   This module exists to provide type information and functions needed by Box.DH. Box.AE is not imported directly by
+   Box.DH to preserve some notion of modularity. If Box.DH should be used with some other module, only Box.PlainDH
+   should have to be edited.
+*)
+module Box.Key
+
+open FStar.HyperHeap
+open FStar.HyperStack
+open FStar.HyperHeap.ST
+open Crypto.Symmetric.Bytes
+
+module MR = FStar.Monotonic.RRef
+module HH = FStar.HyperHeap
+module HS = FStar.HyperStack
+module MM = MonotoneMap
+module SPEC = Spec.SecretBox
+
+assume val is_random: bytes -> Type0
+
+// Have an abstract(?) key type in here with a leak function attached? Then abstract-alias it in the AE module.
+// Then we can use it in other places if we don't idealize.
+// What refinements to have on the leak function?
+
+type id = int
+type nonce = SPEC.nonce
+let noncesize = SPEC.noncelen
+let keysize = SPEC.keylen
+type aes_key = SPEC.key
+type bytes = SPEC.bytes
+type cipher = b:bytes{Seq.length b >= 16 /\ (Seq.length b - 16) / Spec.Salsa20.blocklen < pow2 32}
+
+
+type ae_log_region =
+  r:MR.rid{ extends r root
+            /\ is_eternal_region r
+            /\ is_below r root
+            }
+
+#set-options "--z3rlimit 500 --max_ifuel 2 --max_fuel 0"
+type protected_ae_plain (i:id) = bytes
+type pairtype (i:id)= (cipher*protected_ae_plain i)
+type key_log_key = (nonce*(i:id))
+type key_log_value (i:id) = (cipher*protected_ae_plain i)
+type key_log_range (k:ae_log_key) = ae_log_value (snd k)
+type key_log_inv (f:MM.map' ae_log_key ae_log_range) = True
+
+type key_log (rgn:ae_log_region) =
+  MM.t rgn ae_log_key ae_log_range ae_log_inv
+
+noeq abstract type key (#it:Type0) (id:it) =
+  | Key: rgn:ae_log_region -> log:(ae_log rgn) -> raw:bytes -> key #it id
+
+abstract noeq type key_module (im:index_module) =
+  | KM:
+    key:Type0 ->
+    rgn:ae_log_region ->
+    fresh: (id:it -> Type0) ->
+    honest: (id:it -> Type0) ->
+    honestST: (id:it -> ST bool
+      (requires (fun h0 -> True))
+      (ensures (fun h0 b h1 -> b <==> honest id))) ->
+    dishonest: (id:it -> Type0) ->
+    dishonestST: (id:it -> ST bool
+      (requires (fun h0 -> True))
+      (ensures (fun h0 b h1 -> b <==> dishonest id))) ->
+    make_honest: (id:it -> ST unit
+      (requires (fun h0 -> ~(dishonest id)))
+      (ensures (fun h0 _ h1 -> honest id))) ->
+    make_dishonest: (id:it -> ST unit
+      (requires (fun h0 -> ~(honest id)))
+      (ensures (fun h0 _ h1 -> dishonest id))) ->
+    get_rawGT: (#id:it -> (k:key #it id) -> GTot (b:bytes{k.raw = b})) -> // Returns the raw bytes of the key. Needed for spec of gen/leak/coerce.
+    gen: (id:it -> ST (k:key id)
+      (requires fun h -> honest id)
+      (ensures fun h0 k h1 -> True)) ->
+    coerce: (id:it -> b:bytes -> ST (k:key id)
+      (requires fun h -> ~(honest id))
+      (ensures fun h0 k h1 -> True)) ->  // What requirments for coerce? Determinism?
+    leak: (#id:it -> k:key id -> ST (b:bytes)
+      (requires (fun h -> ~(honest id)))
+      (ensures (fun h0 k h1 -> True))) -> // What requirements here? Inverse of coerce?
+    key_module
+
+val get_region: km:key_module -> ae_log_region
+let get_region km =
+  km.rgn
+
+val getIt: km:key_module -> Type0
+let getIt km =
+  km.it
+
+val honest: km:key_module -> id:km.it -> Type0
+let honest km id =
+  km.honest id
+
+val honestST: km:key_module -> id:km.it -> ST bool
+  (requires (fun h0 -> True))
+  (ensures (fun h0 b h1 -> b <==> honest km id))
+let honestST km id =
+  km.honestST id
+
+
+val dishonest: km:key_module -> id:km.it -> Type0
+let dishonest km id =
+  km.dishonest id
+
+val dishonestST: km:key_module -> id:km.it -> ST bool
+  (requires (fun h0 -> True))
+  (ensures (fun h0 b h1 -> b <==> dishonest km id))
+let dishonestST km id =
+  km.dishonestST id
+
+val make_honest: km:key_module -> id:km.it -> ST unit
+  (requires (fun h0 -> ~(dishonest km id)))
+  (ensures (fun h0 b h1 -> honest km id))
+let make_honest km id =
+  km.make_honest id
+
+val make_dishonest: km:key_module -> id:km.it -> ST unit
+  (requires (fun h0 -> ~(honest km id)))
+  (ensures (fun h0 b h1 -> dishonest km id))
+let make_dishonest km id =
+  km.make_dishonest id
+
+val gen: (km:key_module) -> (id:km.it) -> ST (k:key #km.it id)
+  (requires (fun h0 -> km.fresh id))
+  (ensures (fun h0 k h1 -> True))
+let gen km id =
+  km.gen id
+
+val coerce: (km:key_module) -> (id:km.it) -> (b:bytes) -> ST (k:key #km.it id)
+  (requires (fun h0 -> ~(km.honest id)))
+  (ensures (fun h0 k h1 -> True))
+let coerce km id b =
+  km.coerce id b
+
+val leak: (km:key_module) -> (#id:km.it) -> (k:key id) -> ST (b:bytes)
+  (requires (fun h0 -> ~(km.honest id)))
+  (ensures (fun h0 k h1 -> True))
+let leak km #id k =
+  km.leak k
