secure_api/box/functor_box/Box.Plain.fst
@@ -1,0 +1,77 @@
+(**
+  This module contains the plaintext type of AE and functions to access it.
+*)
+module Box.Plain
+
+open FStar.Seq
+open FStar.HyperHeap
+open FStar.HyperStack
+open FStar.HyperStack.ST
+
+open Box.Flags
+open Box.Indexing
+
+(**
+  The protected plaintext type of AE. It is associated with an id and acts as a wrapper around a protected pkae plaintext.
+  The ids associated with both plaintexts must be equal.
+*)
+
+#set-options "--z3rlimit 300 --max_ifuel 1 --max_fuel 0"
+abstract noeq type plain_module =
+  | PM:
+    plain: (Type0) ->
+    //repr: ((#i:id im) -> (protected_plain_t i) -> (p:plain_type{dishonest im (ID i) \/ not ae_ind_cpa})) ->
+    //coerce: (#i:id im -> plain_type -> (p:protected_plain_t i{dishonest im (ID i) \/ not ae_int_ctxt})) ->
+    length: (plain -> nat) ->
+    plain_module
+
+abstract type protected_plain_t (im:index_module) (pt:Type0) (id:id im) = pt
+
+val index_module_lemma: im:index_module -> i:meta_id im -> ST unit
+  (requires (fun h0 -> registered im i))
+  (ensures (fun h0 _ h1 ->
+    (honest im i ==> (~(dishonest im i) /\ ~(undefined im i)))
+    /\ (dishonest im i ==> (~(honest im i) /\ ~(undefined im i)))
+    /\ (undefined im i ==> (~(honest im i) /\ ~(dishonest im i)))
+  ))
+let index_module_lemma im i =
+  match get_honesty im i with
+  | UNDEFINED ->
+    lemma_undefined_not_others im i
+  | DISHONEST ->
+    lemma_dishonest_not_others im i
+  | HONEST ->
+    lemma_honest_not_others im i
+
+val get_plain: pm:plain_module -> Type0
+let get_plain pm =
+  pm.plain
+
+val repr: #im:index_module -> #pm:plain_module -> #i:id im{dishonest im (ID i) \/ not ae_ind_cpa} -> protected_plain_t im pm.plain i -> (p:pm.plain)
+let repr #im #pm #i p =
+  p
+
+val coerce: #im:index_module -> #pm:plain_module -> #i:id im{dishonest im (ID i) \/ not ae_int_ctxt} -> pm.plain -> (p:protected_plain_t im pm.plain i)
+let coerce #im #pm #i p =
+  p
+
+val length: #im:index_module -> #pm:plain_module -> #i:id im -> (p:protected_plain_t im pm.plain i) -> nat
+let length #im #pm #i p =
+  pm.length p
+
+val rec_repr: #im:index_module ->
+              #inner_pm:plain_module ->
+              #pm:plain_module ->
+              #i:id im{dishonest im (ID i) \/ not ae_ind_cpa} ->
+              p:protected_plain_t im pm.plain i{protected_plain_t im pm.plain i === protected_plain_t im inner_pm.plain i}
+              -> Tot (inner_pm.plain)
+let rec_repr #im #inner_pm #pm #i p =
+  repr #im #inner_pm #i p
+
+val message_wrap: #im:index_module -> #inner_pm:plain_module -> #pm:plain_module -> #i:id im -> p:inner_pm.plain{protected_plain_t im pm.plain i === protected_plain_t im inner_pm.plain i} -> protected_plain_t im pm.plain i
+let message_wrap #im #inner_pm #pm #i p =
+  p
+
+val message_unwrap: #im:index_module -> #inner_pm:plain_module -> #pm:plain_module -> #i:id im -> p:pm.plain{protected_plain_t im pm.plain i === protected_plain_t im inner_pm.plain i} -> protected_plain_t im inner_pm.plain i
+let message_unwrap #im #inner_pm #pm #i p =
+  p
